Rename sigma:Sigma to pstate:PState

Prog.v
@@ -21,135 +21,135 @@ Inductive prog3 : Type -> Type :=
 Definition disk := mem addr block.
 
 (** The state the program manipulates as it executes. *)
-Record Sigma :=
+Record PState :=
   Disks { disk0 : disk;
           disk1 : disk;
           disk2 : disk }.
 
 (** Get a particular disk from a state by id. *)
-Definition disk_id (i:diskId) (sigma:Sigma) : disk :=
+Definition disk_id (i:diskId) (pstate:PState) : disk :=
   match i with
-  | d0 => disk0 sigma
-  | d1 => disk1 sigma
-  | d2 => disk2 sigma
+  | d0 => disk0 pstate
+  | d1 => disk1 pstate
+  | d2 => disk2 pstate
   end.
 
 (** Apply an update function [up] to the disk identified by [i] in the state
-[sigma]. *)
-Definition upd_disk (i:diskId) (sigma:Sigma) (up:disk -> disk) : Sigma :=
+[pstate]. *)
+Definition upd_disk (i:diskId) (pstate:PState) (up:disk -> disk) : PState :=
   match i with
-  | d0 => let 'Disks d_0 d_1 d_2 := sigma in Disks (up d_0) d_1 d_2
-  | d1 => let 'Disks d_0 d_1 d_2 := sigma in Disks d_0 (up d_1) d_2
-  | d2 => let 'Disks d_0 d_1 d_2 := sigma in Disks d_0 d_1 (up d_2)
+  | d0 => let 'Disks d_0 d_1 d_2 := pstate in Disks (up d_0) d_1 d_2
+  | d1 => let 'Disks d_0 d_1 d_2 := pstate in Disks d_0 (up d_1) d_2
+  | d2 => let 'Disks d_0 d_1 d_2 := pstate in Disks d_0 d_1 (up d_2)
   end.
 
 (** A [StepResult] is the result of executing a program - it may give a final
 outcome and return value, or report that the program fails. A third option
 [NonDet] allows a StepResult to not specify any behavior for a program,
 potentially under only certain conditions. *)
-Inductive StepResult Sigma T :=
-| StepTo (v:T) (sigma:Sigma)
+Inductive StepResult PState T :=
+| StepTo (v:T) (pstate:PState)
 | Fails
 | NonDet.
-Arguments Fails {Sigma T}.
-Arguments NonDet {Sigma T}.
+Arguments Fails {PState T}.
+Arguments NonDet {PState T}.
 
 (** [step] gives each primitive operation a semantics by specifying how the
 state is transformed and giving a return value of the appropriate type. *)
-Definition step T (p:prog3 T) (sigma:Sigma) : StepResult Sigma T :=
+Definition step T (p:prog3 T) (pstate:PState) : StepResult PState T :=
   match p with
   | Read i a =>
-    match (disk_id i sigma) a with
-    | Some v => StepTo v sigma
+    match (disk_id i pstate) a with
+    | Some v => StepTo v pstate
     | None => Fails
     end
   | Write i a b =>
-    match (disk_id i sigma) a with
-    | Some _ => let sigma' := upd_disk i sigma (fun d => upd d a b) in
-               StepTo tt sigma'
+    match (disk_id i pstate) a with
+    | Some _ => let pstate' := upd_disk i pstate (fun d => upd d a b) in
+               StepTo tt pstate'
     | None => Fails
     end
-  | Ret v => StepTo v sigma
+  | Ret v => StepTo v pstate
   | Bind _ _ => NonDet
   end.
 
 (** A [Result] is the outcome from running a program. *)
-Inductive Result Sigma T :=
-  (** the program finished, returning v and leaving the state at [sigma] *)
-| Finished (v:T) (sigma:Sigma)
-(** the program could crash at some intermediate point in state [sigma] (the return
+Inductive Result PState T :=
+  (** the program finished, returning v and leaving the state at [pstate] *)
+| Finished (v:T) (pstate:PState)
+(** the program could crash at some intermediate point in state [pstate] (the return
 value is in memory and is thus lost) *)
-| Crashed (sigma:Sigma)
+| Crashed (pstate:PState)
 (** the program failed by attempting some illegal operation, eg, an
 out-of-bounds write *)
 | Failed.
-Arguments Crashed {Sigma T} sigma.
-Arguments Failed {Sigma T}.
+Arguments Crashed {PState T} pstate.
+Arguments Failed {PState T}.
 
 (** Finally [exec] gives the semantics of a whole program. This combines
 behavior of each individual instruction given by [step] with [Bind], which
 sequentially composes programs, and crashes, which can expose any intermediate
 state of a program. *)
-Inductive exec : forall T, prog3 T -> Sigma -> Result Sigma T -> Prop :=
-| ExecStepTo : forall T (p:prog3 T) sigma v sigma',
-    step p sigma = StepTo v sigma' ->
-    exec p sigma (Finished v sigma')
-| ExecStepFail : forall T (p:prog3 T) sigma,
-    step p sigma = Fails ->
-    exec p sigma Failed
-| ExecCrashBefore : forall T (p: prog3 T) sigma,
-    exec p sigma (Crashed sigma)
-| ExecCrashAfter : forall T (p: prog3 T) sigma v sigma',
-    step p sigma = StepTo v sigma' ->
-    exec p sigma (Crashed sigma')
+Inductive exec : forall T, prog3 T -> PState -> Result PState T -> Prop :=
+| ExecStepTo : forall T (p:prog3 T) pstate v pstate',
+    step p pstate = StepTo v pstate' ->
+    exec p pstate (Finished v pstate')
+| ExecStepFail : forall T (p:prog3 T) pstate,
+    step p pstate = Fails ->
+    exec p pstate Failed
+| ExecCrashBefore : forall T (p: prog3 T) pstate,
+    exec p pstate (Crashed pstate)
+| ExecCrashAfter : forall T (p: prog3 T) pstate v pstate',
+    step p pstate = StepTo v pstate' ->
+    exec p pstate (Crashed pstate')
 | ExecBindFinished : forall T T' (p: prog3 T) (p': T -> prog3 T')
-                     sigma v sigma' r,
-    exec p sigma (Finished v sigma') ->
-    exec (p' v) sigma' r ->
-    exec (Bind p p') sigma r
+                     pstate v pstate' r,
+    exec p pstate (Finished v pstate') ->
+    exec (p' v) pstate' r ->
+    exec (Bind p p') pstate r
 | ExecBindCrashed : forall T T' (p: prog3 T) (p': T -> prog3 T')
-                   sigma sigma',
+                   pstate pstate',
     (* Note: this introduces some executions redundant with ExecCrashBefore,
     since the bind can directly crash using ExecCrashBefore or its first
     component can use ExecCrashBefore and then the bind uses this
     constructor. *)
-    exec p sigma (Crashed sigma') ->
-    exec (Bind p p') sigma (Crashed sigma')
+    exec p pstate (Crashed pstate') ->
+    exec (Bind p p') pstate (Crashed pstate')
 | ExecBindFailed : forall T T' (p: prog3 T) (p': T -> prog3 T')
-                   sigma,
-    exec p sigma Failed ->
-    exec (Bind p p') sigma Failed.
+                   pstate,
+    exec p pstate Failed ->
+    exec (Bind p p') pstate Failed.
 
 (** analogous to [Result] for recovery *)
-Inductive RResult Sigma T R :=
-| RFinished (v:T) (sigma:Sigma)
-| Recovered (v:R) (sigma:Sigma)
+Inductive RResult PState T R :=
+| RFinished (v:T) (pstate:PState)
+| Recovered (v:R) (pstate:PState)
 | RFailed.
 
-Arguments RFinished {Sigma T R} v sigma.
-Arguments Recovered {Sigma T R} v sigma.
-Arguments RFailed {Sigma T R}.
+Arguments RFinished {PState T R} v pstate.
+Arguments Recovered {PState T R} v pstate.
+Arguments RFailed {PState T R}.
 
 (** mark a recovery result as always being recovered, since it was executed
 after a crash *)
-Definition to_recovered {Sigma T R} (r:RResult Sigma R R) : RResult Sigma T R :=
+Definition to_recovered {PState T R} (r:RResult PState R R) : RResult PState T R :=
   match r with
-  | RFinished v sigma => Recovered v sigma
-  | Recovered v sigma => Recovered v sigma
+  | RFinished v pstate => Recovered v pstate
+  | Recovered v pstate => Recovered v pstate
   | RFailed => RFailed
   end.
 
-Inductive exec_recover T R : prog3 T -> prog3 R -> Sigma -> RResult Sigma T R -> Prop :=
-| RExec : forall (p:prog3 T) (rec:prog3 R) sigma v sigma',
-    exec p sigma (Finished v sigma') ->
-    exec_recover p rec sigma (RFinished v sigma')
-| RExecFailed : forall (p:prog3 T) (rec:prog3 R) sigma,
-    exec p sigma Failed ->
-    exec_recover p rec sigma RFailed
-| RExecCrash : forall (p:prog3 T) (rec:prog3 R) sigma sigma' r,
-    exec p sigma (Crashed sigma') ->
-    exec_recover (T:=R) rec rec sigma' r ->
-    exec_recover p rec sigma (to_recovered r).
+Inductive exec_recover T R : prog3 T -> prog3 R -> PState -> RResult PState T R -> Prop :=
+| RExec : forall (p:prog3 T) (rec:prog3 R) pstate v pstate',
+    exec p pstate (Finished v pstate') ->
+    exec_recover p rec pstate (RFinished v pstate')
+| RExecFailed : forall (p:prog3 T) (rec:prog3 R) pstate,
+    exec p pstate Failed ->
+    exec_recover p rec pstate RFailed
+| RExecCrash : forall (p:prog3 T) (rec:prog3 R) pstate pstate' r,
+    exec p pstate (Crashed pstate') ->
+    exec_recover (T:=R) rec rec pstate' r ->
+    exec_recover p rec pstate (to_recovered r).
 
 Notation "x <- p1 ; p2" := (Bind p1 (fun x => p2))
                             (at level 60, right associativity).
@@ -158,5 +158,5 @@ Notation "'do' x .. y <- p1 ; p2" := (Bind p1 (fun x => .. (fun y => p2) ..))
                                        x binder, y binder, only parsing).
 
 (* Local Variables: *)
-(* company-coq-local-symbols: (("Sigma" . ?Σ) ("sigma" . ?σ) ("sigma'" . (?σ (Br . Bl) ?'))) *)
+(* company-coq-local-symbols: (("PState" . ?Σ) ("pstate" . ?σ) ("pstate'" . (?σ (Br . Bl) ?'))) *)
 (* End: *)
